backend/CminorSel.v
@@ -446,7 +446,7 @@ Inductive step: state -> trace -> state -> Prop :=
 
   | step_internal_function: forall f vargs k m m' m'' sp e id,
       Mem.alloc m 0 f.(fn_stackspace) = (m', sp) ->
-      Mem.record_frame m' (Memory.mk_frame (fn_stack_requirements id)) = Some m'' ->
+      Mem.record_frame m' (Memory.mk_frame sp (fn_stack_requirements id)) = Some m'' ->
       set_locals f.(fn_vars) (set_params vargs f.(fn_params)) = e ->
       step (Callstate (Internal f) vargs k m id)
         E0 (State f f.(fn_body) k (Vptr sp Ptrofs.zero) e m'')
